split up example into their own files

VerifiedFilter/Grammar/Grammar.lean
@@ -1,11 +1,21 @@
-import VerifiedFilter.Std.Hedge
-import VerifiedFilter.Std.List
-import VerifiedFilter.Std.Vector
+-- Grammar defines a symbolic regular hedge grammar.
 
-import VerifiedFilter.Pred.AnyEq
 import VerifiedFilter.Regex.Regex
-import VerifiedFilter.Regex.Lang
-import VerifiedFilter.Grammar.Types
+
+-- ## Definition 3.2.3: Regular Hedge Grammar
+--   𝐺 = (𝑁, 𝑇, 𝑆, 𝑃)
+--   𝑁 a finite set of non-terminals
+--   𝑇 a finite set of terminals
+--   𝑆 the start symbol of a regular hedge grammar is a regular expression comprising pairs of nonterminals and terminals (a regular expression over N × T)
+--   𝑃 a set of production rules of a regular hedge grammar are of the form X → r such that r is a regular expression over N × T.
+
+-- Ref is a non-terminal, where n represents the number of non-terminals
+abbrev Ref (n: Nat) := Fin n
+
+-- symbolic regular hedge grammar
+structure Grammar (n: Nat) (φ: Type) where
+  start: Regex (φ × Ref n)
+  prods: Vector (Regex (φ × Ref n)) n
 
 namespace Grammar
 
@@ -20,42 +30,3 @@ def emptyset: Grammar 0 φ :=
 
 def emptystr: Grammar 0 φ :=
   singleton Regex.emptystr
-
-example: Grammar 2 String := Grammar.mk
-  (start := Regex.symbol ("title", 0))
-  (prods := #v[
-    Regex.symbol ("verified derivatives", 1),
-    Regex.emptystr,
-  ])
-
-open Pred
-
-example : Grammar 5 (AnyEq.Pred String) := Grammar.mk
-  -- start := ("html", Html)
-  (start := Regex.symbol (AnyEq.Pred.eq "html", 0))
-  -- production rules
-  (prods := #v[
-    -- Html -> ("head", Head) · ("body", Body)
-    Regex.concat
-      (Regex.symbol (AnyEq.Pred.eq "head", 1))
-      (Regex.symbol (AnyEq.Pred.eq "body", 2))
-    -- Head -> ("title", Text) | ε
-    , Regex.or
-      (Regex.symbol (AnyEq.Pred.eq "title", 3))
-      Regex.emptystr
-    -- Body -> ("p", Text)*
-    , Regex.star (Regex.symbol (AnyEq.Pred.eq "p", 3))
-    -- Text -> (., Empty)
-    , Regex.symbol (AnyEq.Pred.any, 4)
-    -- Empty -> ε
-    , Regex.emptystr
-  ])
-
-private def example_grammar: Grammar 1 (AnyEq.Pred Char) :=
-  Grammar.mk
-    (Regex.or Regex.emptystr (Regex.symbol (AnyEq.Pred.eq 'a', 0)))
-    #v[Regex.emptystr]
-
-#guard
-  example_grammar.lookup (Fin.mk 0 (by omega))
-  = Regex.emptystr
