VerifiedFilter/Grammar/GrammarExamples.lean
@@ -1,0 +1,51 @@
+-- examples of a symbolic regular hedge grammar using Pred.
+
+import VerifiedFilter.Std.Hedge
+import VerifiedFilter.Std.List
+import VerifiedFilter.Std.Vector
+
+import VerifiedFilter.Pred.AnyEq
+import VerifiedFilter.Regex.Regex
+import VerifiedFilter.Regex.Lang
+import VerifiedFilter.Grammar.Grammar
+
+namespace Grammar
+
+example: Grammar 2 String := Grammar.mk
+  (start := Regex.symbol ("title", 0))
+  (prods := #v[
+    Regex.symbol ("verified derivatives", 1),
+    Regex.emptystr,
+  ])
+
+open Pred
+
+example : Grammar 5 (AnyEq.Pred String) := Grammar.mk
+  -- start := ("html", Html)
+  (start := Regex.symbol (AnyEq.Pred.eq "html", 0))
+  -- production rules
+  (prods := #v[
+    -- Html -> ("head", Head) · ("body", Body)
+    Regex.concat
+      (Regex.symbol (AnyEq.Pred.eq "head", 1))
+      (Regex.symbol (AnyEq.Pred.eq "body", 2))
+    -- Head -> ("title", Text) | ε
+    , Regex.or
+      (Regex.symbol (AnyEq.Pred.eq "title", 3))
+      Regex.emptystr
+    -- Body -> ("p", Text)*
+    , Regex.star (Regex.symbol (AnyEq.Pred.eq "p", 3))
+    -- Text -> (., Empty)
+    , Regex.symbol (AnyEq.Pred.any, 4)
+    -- Empty -> ε
+    , Regex.emptystr
+  ])
+
+private def example_grammar: Grammar 1 (AnyEq.Pred Char) :=
+  Grammar.mk
+    (Regex.or Regex.emptystr (Regex.symbol (AnyEq.Pred.eq 'a', 0)))
+    #v[Regex.emptystr]
+
+#guard
+  example_grammar.lookup (Fin.mk 0 (by omega))
+  = Regex.emptystr
