VerifiedFilter/Grammar/JSONSchemaExamples.lean
@@ -1,0 +1,186 @@
+import VerifiedFilter.Std.Hedge
+
+import VerifiedFilter.Grammar.Grammar
+import VerifiedFilter.Grammar.JSONSchema
+
+import VerifiedFilter.Pred.AnyEq
+import VerifiedFilter.Pred.Compare
+
+
+-- Tests
+
+namespace Grammar.JSONSchema
+
+open Pred
+open Hedge
+
+def run [DecidableEq α] (G: Grammar n (AnyEq.Pred α)) (nodes: Hedge α): Bool :=
+  validate G AnyEq.Pred.evalb nodes
+
+#guard run
+  (Grammar.singleton Regex.emptyset)
+  [node "a" [node "b" [], node "c" [node "d" []]]] =
+  false
+
+#guard run
+  (Grammar.mk (n := 1)
+    (Regex.symbol (AnyEq.Pred.eq "a", 0))
+    #v[Regex.emptystr]
+  )
+  [node "a" []] =
+  true
+
+#guard run
+  (Grammar.mk (n := 1)
+    (Regex.symbol (AnyEq.Pred.eq "a", 0))
+    #v[Regex.emptystr]
+  )
+  [node "a" [node "b" []]] =
+  false
+
+#guard run
+  (Grammar.mk (n := 2)
+    (Regex.symbol (AnyEq.Pred.eq "a", 0))
+    #v[
+      (Regex.symbol (AnyEq.Pred.eq "b", 1))
+      , Regex.emptystr
+    ]
+  )
+  [node "a" [node "b" []]]
+  = true
+
+#guard run
+  (Grammar.mk (n := 2)
+    (Regex.symbol (AnyEq.Pred.eq "a", 0))
+    #v[
+      (Regex.concat
+        (Regex.symbol (AnyEq.Pred.eq "b", 1))
+        (Regex.symbol (AnyEq.Pred.eq "c", 1))
+      )
+      , Regex.emptystr
+    ]
+  )
+  [node "a" [node "b" [], node "c" []]] =
+  true
+
+#guard run
+  (Grammar.mk (n := 3)
+    (Regex.symbol (AnyEq.Pred.eq "a", 0))
+    #v[
+      (Regex.concat
+        (Regex.symbol (AnyEq.Pred.eq "b", 1))
+        (Regex.symbol (AnyEq.Pred.eq "c", 2))
+      )
+      , Regex.emptystr
+      , (Regex.symbol (AnyEq.Pred.eq ("d"), 1))
+    ]
+  )
+  [node "a" [node "b" [], node "c" [node "d" []]]] =
+  true
+
+-- modified example from https://books.xmlschemata.org/relaxng/relax-CHP-5-SECT-4.html
+
+private def example_grammar_library: Grammar 5 (Option String) :=
+  Grammar.mk
+    (start := Regex.symbol (some "library", 0))
+    (prods := #v[
+      Regex.oneOrMore (Regex.symbol (some "book", 1)),
+      Regex.concat
+        (Regex.symbol (some "isbn", 3))
+        (Regex.concat
+          (Regex.symbol (some "title", 3))
+          (Regex.oneOrMore (Regex.symbol (some "author", 2)))
+        ),
+      Regex.concat
+        (Regex.symbol (some "name", 3))
+        (Regex.optional (Regex.symbol (some "born", 3))),
+      Regex.symbol (Option.none, 4),
+      Regex.emptystr
+    ])
+
+#guard validate
+  example_grammar_library
+  (fun s a =>
+    match s with
+    | Option.none => true
+    | Option.some s' => s' == a
+  )
+  [node "library"
+    [node "book" [
+      (node "isbn" [node "123" []]),
+      (node "title" [node "numbers" []]),
+      (node "author" [node "name" [node "Brink" []]]),
+      (node "author" [node "name" [node "Paul" []], node "born" [node "July" []]])
+    ]]
+  ]
+  = true
+
+-- no authors fails
+#guard validate
+  example_grammar_library
+  (fun s a =>
+    match s with
+    | Option.none => true
+    | Option.some s' => s' == a
+  )
+  [node "library"
+    [node "book" [
+      (node "isbn" [node "456" []]),
+      (node "title" [node "numbers" []])
+    ]]
+  ]
+  = false
+
+-- modified example from Taxonomy of XML Section 6.5
+
+private def example_grammar_doc: Grammar 3 String :=
+  Grammar.mk (start := Regex.symbol ("doc", 0))
+    (prods := #v[
+      Regex.oneOrMore (Regex.symbol ("para", 1)),
+      Regex.symbol ("pcdata", 2),
+      Regex.emptystr,
+    ])
+
+#guard validate example_grammar_doc (· == ·)
+  [node "doc" [node "para" [node "pcdata" []]]]
+  = true
+
+#guard validate example_grammar_doc (· == ·)
+  [node "doc" [node "para" []]]
+  = false
+
+#guard validate example_grammar_doc (· == ·)
+  [node "doc" [node "para" [node "pcdata" []], node "para" [node "pcdata" []]]]
+  = true
+
+#guard validate example_grammar_doc (· == ·)
+  [node "doc" [node "para" [node "pcdata" []], node "para" [node "pcdata" []], node "para" [node "pcdata" []]]]
+  = true
+
+-- modified example from Taxonomy of XML Section 7.1
+private def example_grammar_sec: Grammar 2 String :=
+  Grammar.mk
+    (start := Regex.oneOrMore (Regex.symbol ("sec", 0)))
+    (prods := #v[
+      Regex.oneOrMore (Regex.or
+        (Regex.symbol ("sec", 0))
+        (Regex.symbol ("p", 1))
+      ),
+      Regex.emptystr
+    ])
+
+#guard validate example_grammar_sec (· == ·)
+  [node "sec" [node "p" []]]
+  = true
+
+#guard validate example_grammar_sec (· == ·)
+  [node "sec" [node "p" []], node "sec" [node "sec" [node "p" []], node "sec" [node "p" []], node "sec" [node "p" []]]]
+  = true
+
+#guard validate example_grammar_sec (· == ·)
+  [node "sec" []]
+  = false
+
+#guard validate example_grammar_sec (· == ·)
+  [node "p" []]
+  = false
