VerifiedFilter/Grammar/KatydidExamples.lean
@@ -1,0 +1,359 @@
+import VerifiedFilter.Std.Hedge
+
+import VerifiedFilter.Grammar.Grammar
+import VerifiedFilter.Grammar.Katydid
+
+import VerifiedFilter.Pred.AnyEq
+import VerifiedFilter.Pred.Compare
+
+open Hedge
+
+-- Tests
+
+namespace Grammar.Katydid
+
+open Pred
+
+def run [DecidableEq α] (G: Grammar n (AnyEq.Pred α)) (nodes: Hedge α): Bool :=
+  validate G AnyEq.Pred.evalb nodes
+
+abbrev contains (r: Regex σ) := Regex.contains r
+abbrev symbol (s: σ) := Regex.symbol s
+abbrev emptystr : Regex σ := Regex.emptystr
+abbrev interleave (r1 r2: Regex σ) := Regex.interleave r1 r2
+abbrev or (r1 r2: Regex σ) := Regex.or r1 r2
+abbrev and (r1 r2: Regex σ) := Regex.and r1 r2
+abbrev optional (r: Regex σ) := Regex.optional r
+abbrev starAny: Regex σ := Regex.starAny
+
+#guard run
+  (Grammar.singleton Regex.emptyset)
+  [node "a" [node "b" [], node "c" [node "d" []]]] =
+  false
+
+#guard run
+  (Grammar.mk (n := 1)
+    (Regex.symbol (AnyEq.Pred.eq "a", 0))
+    #v[Regex.emptystr]
+  )
+  [node "a" []] =
+  true
+
+#guard run
+  (Grammar.mk (n := 1)
+    (Regex.symbol (AnyEq.Pred.eq "a", 0))
+    #v[Regex.emptystr]
+  )
+  [node "a" [node "b" []]] =
+  false
+
+#guard run
+  (Grammar.mk (n := 2)
+    (Regex.symbol (AnyEq.Pred.eq "a", 0))
+    #v[
+      (Regex.symbol (AnyEq.Pred.eq "b", 1))
+      , Regex.emptystr
+    ]
+  )
+  [node "a" [node "b" []]]
+  = true
+
+#guard run
+  (Grammar.mk (n := 2)
+    (Regex.symbol (AnyEq.Pred.eq "a", 0))
+    #v[
+      (Regex.concat
+        (Regex.symbol (AnyEq.Pred.eq "b", 1))
+        (Regex.symbol (AnyEq.Pred.eq "c", 1))
+      )
+      , Regex.emptystr
+    ]
+  )
+  [node "a" [node "b" [], node "c" []]] =
+  true
+
+#guard run
+  (Grammar.mk (n := 3)
+    (Regex.symbol (AnyEq.Pred.eq "a", 0))
+    #v[
+      (Regex.concat
+        (Regex.symbol (AnyEq.Pred.eq "b", 1))
+        (Regex.symbol (AnyEq.Pred.eq "c", 2))
+      )
+      , Regex.emptystr
+      , (Regex.symbol (AnyEq.Pred.eq ("d"), 1))
+    ]
+  )
+  [node "a" [node "b" [], node "c" [node "d" []]]] =
+  true
+
+-- modified example from https://books.xmlschemata.org/relaxng/relax-CHP-5-SECT-4.html
+
+private def example_grammar_library: Grammar 5 (Option String) :=
+  Grammar.mk
+    (start := Regex.symbol (some "library", 0))
+    (prods := #v[
+      Regex.oneOrMore (Regex.symbol (some "book", 1)),
+      Regex.concat
+        (Regex.symbol (some "isbn", 3))
+        (Regex.concat
+          (Regex.symbol (some "title", 3))
+          (Regex.oneOrMore (Regex.symbol (some "author", 2)))
+        ),
+      Regex.concat
+        (Regex.symbol (some "name", 3))
+        (Regex.optional (Regex.symbol (some "born", 3))),
+      Regex.symbol (Option.none, 4),
+      Regex.emptystr
+    ])
+
+#guard validate
+  example_grammar_library
+  (fun s a =>
+    match s with
+    | Option.none => true
+    | Option.some s' => s' == a
+  )
+  [node "library"
+    [node "book" [
+      (node "isbn" [node "123" []]),
+      (node "title" [node "numbers" []]),
+      (node "author" [node "name" [node "Brink" []]]),
+      (node "author" [node "name" [node "Paul" []], node "born" [node "July" []]])
+    ]]
+  ]
+  = true
+
+-- no authors fails
+#guard validate
+  example_grammar_library
+  (fun s a =>
+    match s with
+    | Option.none => true
+    | Option.some s' => s' == a
+  )
+  [node "library"
+    [node "book" [
+      (node "isbn" [node "456" []]),
+      (node "title" [node "numbers" []])
+    ]]
+  ]
+  = false
+
+-- modified example from Taxonomy of XML Section 6.5
+
+private def example_grammar_doc65: Grammar 3 String :=
+  Grammar.mk (start := Regex.symbol ("doc", 0))
+    (prods := #v[
+      Regex.oneOrMore (Regex.symbol ("para", 1)),
+      Regex.symbol ("pcdata", 2),
+      Regex.emptystr,
+    ])
+
+#guard validate example_grammar_doc65 (· == ·)
+  [node "doc" [node "para" [node "pcdata" []]]]
+  = true
+
+#guard validate example_grammar_doc65 (· == ·)
+  [node "doc" [node "para" []]]
+  = false
+
+#guard validate example_grammar_doc65 (· == ·)
+  [node "doc" [node "para" [node "pcdata" []], node "para" [node "pcdata" []]]]
+  = true
+
+#guard validate example_grammar_doc65 (· == ·)
+  [node "doc" [node "para" [node "pcdata" []], node "para" [node "pcdata" []], node "para" [node "pcdata" []]]]
+  = true
+
+-- even more modified version of example from Taxonomy of XML Section 6.5
+
+open Pred.AnyEq
+
+private def example_grammar_doc: Grammar 3 (Pred String) :=
+  Grammar.mk (start := Regex.symbol (Pred.eq "doc", 0))
+    (prods := #v[
+      Regex.oneOrMore (Regex.symbol (Pred.eq "p", 1)),
+      Regex.symbol (Pred.any, 2),
+      Regex.emptystr,
+    ])
+
+#guard validate example_grammar_doc Pred.evalb
+  [node "doc" [node "p" [node "pcdata" []]]]
+  = true
+
+#guard validate example_grammar_doc Pred.evalb
+  [node "doc" [node "p" []]]
+  = false
+
+#guard validate example_grammar_doc Pred.evalb
+  [node "doc" [node "p" [node "pcdata" []], node "p" [node "br" []]]]
+  = true
+
+#guard validate example_grammar_doc Pred.evalb
+  [node "doc" [node "p" [node "pcdata" []], node "p" [node "br" []], node "p" [node "pcdata" []]]]
+  = true
+
+-- modified example from Taxonomy of XML Section 7.1
+private def example_grammar_sec: Grammar 2 String :=
+  Grammar.mk
+    (start := Regex.oneOrMore (Regex.symbol ("sec", 0)))
+    (prods := #v[
+      Regex.oneOrMore (Regex.or
+        (Regex.symbol ("sec", 0))
+        (Regex.symbol ("p", 1))
+      ),
+      Regex.emptystr
+    ])
+
+#guard validate example_grammar_sec (· == ·)
+  [node "sec" [node "p" []]]
+  = true
+
+#guard validate example_grammar_sec (· == ·)
+  [node "sec" [node "p" []], node "sec" [node "sec" [node "p" []], node "sec" [node "p" []], node "sec" [node "p" []]]]
+  = true
+
+#guard validate example_grammar_sec (· == ·)
+  [node "sec" []]
+  = false
+
+#guard validate example_grammar_sec (· == ·)
+  [node "p" []]
+  = false
+
+private def example_benchmark_nested_contains: Grammar 3 String :=
+  mk (contains (symbol ("A",0))) #v[contains (symbol ("B",1)), symbol ("C",2), emptystr]
+
+#guard validate example_benchmark_nested_contains (· == ·)
+  [node "A" [node "B" [node "C" []]]]
+
+#guard validate example_benchmark_nested_contains (· == ·)
+  [node "a" [], node "A" [node "B" [node "D" []], node "B" [node "C" []], node "B" [node "D" []]], node "a" []]
+
+#guard validate example_benchmark_nested_contains (· == ·)
+  [node "a" [node "B" [node "C" []]], node "A" [node "D" [node "C" []], node "B" [node "D" []], node "D" [node "D" []]], node "a" []]
+  = false
+
+private def example_interleave: Grammar 5 String :=
+  mk (interleave (symbol ("A",0)) (interleave (symbol ("B",1)) (optional (symbol ("C",2))))) #v[
+    interleave (symbol ("A1", 3)) (symbol ("A2",3)),
+    interleave (symbol ("Bb", 3)) starAny,
+    contains (symbol ("Cc", 3)),
+    symbol ("t", 4), emptystr]
+
+#guard validate example_interleave (· == ·)
+  [node "A" [node "A1" [node "t" []], node "A2" [node "t" []]], node "B" [node "B2" [node "t" []], node "Bb" [node "t" []]]]
+
+#guard validate example_interleave (· == ·)
+  [node "D" [], node "A" [node "A1" [node "t" []], node "A2" [node "t" []]], node "B" [node "B2" [node "t" []], node "Bb" [node "t" []]]]
+  = false
+
+#guard validate example_interleave (· == ·)
+  [node "B" [node "B1" [node "t" []], node "B2" [node "t" []], node "Bb" [node "t" []]], node "A" [node "A1" [node "t" []], node "A2" [node "t" []]]]
+  = true
+
+#guard validate example_interleave (· == ·)
+  [
+    node "B" [node "B1" [node "t" []], node "Bb" [node "t" []]],
+    node "C" [node "C1" [node "t" []], node "Cc" [node "t" []], node "C2" [node "t" []]],
+    node "A" [node "A1" [node "t" []], node "A2" [node "t" []]]
+  ]
+  = true
+
+#guard validate example_interleave (· == ·)
+  [
+    node "B" [node "B2" [node "t" []], node "Bb" [node "t" []]],
+    node "A" [node "C1" [node "t" []], node "Cc" [node "t" []], node "C2" [node "t" []]],
+    node "A" [node "A1" [node "t" []], node "A2" [node "t" []]]
+  ]
+  = false
+
+#guard validate example_interleave (· == ·)
+  [
+    node "B" [node "B2" [node "t" []], node "Bb" [node "t" []]],
+    node "C" [node "C1" [node "t" []], node "Cc" [node "g" []], node "C2" [node "t" []]],
+    node "A" [node "A1" [node "t" []], node "A2" [node "t" []]]
+  ]
+  = false
+
+-- Benchmark tests
+
+def eq (v: α × Fin n) := symbol (Pred.Compare.Pred.eq v.1, v.2)
+def field (v: α × Fin n) := contains (symbol (Pred.Compare.Pred.eq v.1, v.2))
+
+def simple: Grammar 2 (Pred.Compare.Pred String) :=
+  mk (field ("Category", 1)) #v[emptystr, eq ("Computer Science", 0)]
+
+#guard validate simple Pred.Compare.Pred.evalb
+  [node "Category" [node "Computer Science" []]]
+
+#guard validate simple Pred.Compare.Pred.evalb
+  [node "Name" [node "ITP" []], node "Category" [node "Computer Science" []]]
+
+#guard validate simple Pred.Compare.Pred.evalb
+  [node "Name" [node "ICFP" []], node "Category" [node "Functional Programming" []]]
+  = false
+
+def complex : Grammar 7 (Pred.Compare.Pred String) :=
+  mk (interleave (eq ("Due", 1)) (interleave (eq ("Loc", 5)) starAny)) #v[emptystr,
+    or (field ("Year", 2)) (and (field ("Year", 3)) (field ("Month", 4))),
+    eq ("2026", 0), eq ("2025", 0), symbol (Pred.Compare.Pred.ge "10", 0),
+    field ("Cont", 6), eq ("EU", 0),
+  ]
+
+#guard validate complex Pred.Compare.Pred.evalb
+  [
+    node "Name" [node "ITP" []],
+    node "Loc" [
+      node "Cont" [node "EU" []],
+      node "City" [node "Lisbon" []]
+    ],
+    node "Due" [
+      node "Year" [node "2026" []],
+      node "Month" [node "02" []],
+      node "Day" [node "19" []],
+    ],
+  ]
+
+#guard validate complex Pred.Compare.Pred.evalb
+  [
+    node "Name" [node "ITP" []],
+    node "Loc" [
+      node "Cont" [node "EU" []],
+      node "City" [node "Amsterdam" []]
+    ],
+    node "Due" [
+      node "Year" [node "2025" []],
+      node "Month" [node "11" []],
+      node "Day" [node "19" []],
+    ],
+  ]
+
+#guard validate complex Pred.Compare.Pred.evalb
+  [
+    node "Name" [node "ITP" []],
+    node "Loc" [
+      node "Cont" [node "EU" []],
+    ],
+    node "Due" [
+      node "Y" [node "2027" []],
+      node "Month" [node "02" []],
+      node "Day" [node "19" []],
+    ],
+  ]
+  = false
+
+#guard validate complex Pred.Compare.Pred.evalb
+  [
+    node "Name" [node "ITP" []],
+    node "Loc" [
+      node "Cont" [node "AN" []],
+    ],
+    node "Due" [
+      node "Y" [node "2026" []],
+      node "Month" [node "02" []],
+      node "Day" [node "19" []],
+    ],
+  ]
+  = false
