VerifiedFilter/Grammar/Memoize/StateMemoizeExamples.lean
@@ -1,0 +1,112 @@
+import VerifiedFilter.Std.Hedge
+
+import VerifiedFilter.Regex.Memoize.StateMemoize
+
+import VerifiedFilter.Grammar.Grammar
+import VerifiedFilter.Grammar.Memoize.StateMemoize
+
+import VerifiedFilter.Pred.AnyEq
+import VerifiedFilter.Pred.Compare
+
+open Hedge
+open Regex.Memoize
+open Pred
+
+def validate [DecidableEq φ] [Hashable φ] (G: Grammar n φ) (Φ: φ -> α -> Bool) (nodes: Hedge α): Bool :=
+  StateMemoize.Grammar.validate.run memoizeState.init G Φ nodes
+
+def filter [DecidableEq φ] [Hashable φ] (G: Grammar n φ) (Φ: φ -> α -> Bool) (hedges: List (Hedge α)): List (Hedge α) :=
+  StateMemoize.Grammar.filter.run memoizeState.init G Φ hedges
+
+abbrev contains (r: Regex σ) := Regex.contains r
+abbrev symbol (s: σ) := Regex.symbol s
+abbrev emptystr : Regex σ := Regex.emptystr
+abbrev interleave (r1 r2: Regex σ) := Regex.interleave r1 r2
+abbrev or (r1 r2: Regex σ) := Regex.or r1 r2
+abbrev and (r1 r2: Regex σ) := Regex.and r1 r2
+abbrev starAny: Regex σ := Regex.starAny
+
+def eq (v: α × Fin n) := symbol (Pred.Compare.Pred.eq v.1, v.2)
+def field (v: α × Fin n) := contains (symbol (Pred.Compare.Pred.eq v.1, v.2))
+
+def simple: Grammar 2 (Pred.Compare.Pred String) :=
+  Grammar.mk (field ("Category", 1)) #v[emptystr, eq ("Computer Science", 0)]
+
+#guard validate simple Pred.Compare.Pred.evalb
+  [node "Category" [node "Computer Science" []]]
+
+#guard validate simple Pred.Compare.Pred.evalb
+  [node "Name" [node "ITP" []], node "Category" [node "Computer Science" []]]
+
+#guard validate simple Pred.Compare.Pred.evalb
+  [node "Name" [node "ICFP" []], node "Category" [node "Functional Programming" []]]
+  = false
+
+def complex : Grammar 7 (Pred.Compare.Pred String) :=
+  Grammar.mk (interleave (eq ("Due", 1)) (interleave (eq ("Loc", 5)) starAny)) #v[emptystr,
+    or (field ("Year", 2)) (and (field ("Year", 3)) (field ("Month", 4))),
+    eq ("2026", 0), eq ("2025", 0), symbol (Pred.Compare.Pred.ge "10", 0),
+    field ("Cont", 6), eq ("EU", 0),
+  ]
+
+private def itp_2026 :=
+  [
+    node "Name" [node "ITP" []],
+    node "Loc" [
+      node "Cont" [node "EU" []],
+      node "City" [node "Lisbon" []]
+    ],
+    node "Due" [
+      node "Year" [node "2026" []],
+      node "Month" [node "02" []],
+      node "Day" [node "19" []],
+    ],
+  ]
+
+#guard validate complex Pred.Compare.Pred.evalb itp_2026
+
+private def itp_late_2025 :=
+  [
+    node "Name" [node "ITP" []],
+    node "Loc" [
+      node "Cont" [node "EU" []],
+      node "City" [node "Amsterdam" []]
+    ],
+    node "Due" [
+      node "Year" [node "2025" []],
+      node "Month" [node "11" []],
+      node "Day" [node "19" []],
+    ],
+  ]
+
+#guard validate complex Pred.Compare.Pred.evalb itp_late_2025
+
+private def itp_2027 := [
+    node "Name" [node "ITP" []],
+    node "Loc" [
+      node "Cont" [node "EU" []],
+    ],
+    node "Due" [
+      node "Y" [node "2027" []],
+      node "Month" [node "02" []],
+      node "Day" [node "19" []],
+    ],
+  ]
+
+#guard validate complex Pred.Compare.Pred.evalb itp_2027 = false
+
+private def itp_antarctia := [
+    node "Name" [node "ITP" []],
+    node "Loc" [
+      node "Cont" [node "AN" []],
+    ],
+    node "Due" [
+      node "Y" [node "2026" []],
+      node "Month" [node "02" []],
+      node "Day" [node "19" []],
+    ],
+  ]
+
+#guard validate complex Pred.Compare.Pred.evalb itp_antarctia = false
+
+#guard filter complex Pred.Compare.Pred.evalb [itp_2026, itp_late_2025, itp_2027, itp_antarctia] = [itp_2026, itp_late_2025]
