VerifiedFilter/Grammar/Memoize/Readme.md
@@ -1,0 +1,7 @@
+# Memoize
+
+This folder contains the optimized Katydid algorithm with memoization including proofs of correctness for derive, validate and filter.
+
+* [Memoize](./Memoize.lean) contains the algorithm used by derive, validate and filter.
+* [StateMemoize](./StateMemoize.lean) contains proofs of correctness via instantiating the memoize algorithm with the state monad, for derive, validate and filter.
+* [StateMemoizeExamples](./StateMemoizeExamples.lean) provides examples of how to use StateMemoize to filter efficiently.
