VerifiedFilter/Regex/Readme.md
@@ -1,13 +1,15 @@
 # Regex
 
 In this folder we define a regular expression types, derivatives, validation and filtering algorithms.
-This includes:
 
+We define semantics for the regular expression language in [Lang](./Lang.lean).
+
+The create several implementations of regular expression algorithms:
 * A regular expression over [Char](./Char.lean) and the equivalence proof to symbolic regular expressions.
-* Symbolic regular expressions [Regex](./Regex.lean) with the usual derive, validate and filter functions and proofs of their correctness.
+* Symbolic regular expressions [Regex](./Regex.lean) with the usual derive, validate and filter functions and proofs of their correctness, based on the denotation that is also found here.
 * The optimized [Katydid](./Katydid.lean) algorithm (without memoization) with derive, validate and filter functions and proofs of their correctness.
-* In the [Memoize](./Memoize/) subfolder we define the optimized Katydid algorithm with memoization.
-* In the [IfExpr](./IfExpr/) subfolder we define an alternative implementation without any heap allocations, but with exponential memoization space blowup.
+* In the [Memoize](./Memoize/Readme.md) subfolder we define the optimized Katydid algorithm with memoization.
+* In the [IfExpr](./IfExpr/Readme.md) subfolder we define an alternative implementation without any heap allocations, but with exponential memoization space blowup.
 
 The Katydid algorithm is built on top of some foundational functions and theorems:
 * [Map](./Map.lean) defines the regular expression as a functor that can be mapped over.
